#+TITLE:Mathematics Cheatsheet
#+AUTHOR:LiquidZulu
#+HTML_HEAD:<link rel="stylesheet" type="text/css" href="file:///e:/emacs/documents/org-css/css/org.css"/>
#+OPTIONS: ^:{}
#+STARTUP: latexpreview
#+begin_comment
/This file is best viewed in [[https://www.gnu.org/software/emacs/][emacs]]!/
#+end_comment

* Calculus
** First Principles
Consider $y = f(x)$ with a chord joining $(a, f(a))$ to $(a+h,f(a+h))$.

The gradient of that chord is:

$$
  \frac{f(a+h) - f(a)}{(a+h) - a} = \frac{f(a+h) - f(a)}{h}
$$

The gradient of the tangent to $f(x)$ at point $a$ (provided it exists) is:

$$
  \lim_{h\rightarrow 0}{\frac{f(a+h) - f(a)}{h}}
$$

** Standard Derivatives, and Combinations Thereof
*** Std

  \begin{array}{ccc|ccc|ccc}
    &
      f(x)  &&&
      f'(x) &&&
      \text{Conditions}
    & \\

    \hline

    &
      x^n      &&&
      nx^{n-1} &&&
      n \ne 0, n\in\mathbb{R}, x\in\mathbb{R}
    & \\

    &
      \text{sin } x &&&
      \text{cos } x &&&
      x\in\mathbb{R}
    & \\

    &
      \text{cos } x  &&&
      -\text{sin } x &&&
      x\in\mathbb{R}
    & \\

    &
      \text{tan } x = \frac{\text{sin } x}{\text{cos } x} &&&
      \text{sec}^2 x                                      &&&
      x\in\mathbb{R}
    & \\

    &
      \arcsin{x} &&&
      \frac{1}{\sqrt{1-x^2}} &&&
      x\in\mathbb{R}\setminus\left\{1\right\}
    & \\

    &
      \arccos{x} &&&
      -\frac{1}{\sqrt{1-x^2}} &&&
      x\in\mathbb{R}\setminus\left\{1\right\}
    & \\

    &
      \arcsin{x} &&&
      \frac{1}{1-x^2} &&&
      x\in\mathbb{R}\setminus\left\{1\right\}
    & \\
  \end{array}

*** (f+g)'
$$
  (f+g)'(a) = f'(a) + g'(a)
$$
*** (cf)'
Given $c$ is a constant:
$$
  (cf)'(a) = cf'(a)
$$
*** (fg)'
$(fg)' = f'g + fg'$
*** (f/g)'
$\left(\frac{f}{g}\right)' = \frac{f'g - fg'}{g^2}$
*** (f(g))'
$(f \circ g)'(a) = f'(g(a)) \cdot g'(a)$
*** (a^f(x))'
$$\ln|a|\cdot a^{f(x)}\cdot f^{\prime}(x)$$
** Standard Integrals, and Combinations Thereof
*** f'(x)/f(x)
$$\int{\frac{f^{\prime}(x)}{f(x)}} \text{d}x = \ln|f(x)| + C$$
** differential equations
*** second order
**** homogenous
$\ddot{x} + a_1\dot{x} + a_0 x = 0$

assume $x\left(t\right) = e^{\lambda t}$:

$$\begin{align}
  \lambda^2 e^{\lambda t} + a_1 \lambda e^{\lambda t} + a_0 e^{\lambda t} &= 0 \\
  \leadsto \lambda^2 + a_1\lambda + a_0 &= 0
\end{align}$$

where this quatratic in \lambda is the "characteristic equation"

1. $\lambda_1$ and $\lambda_2$ are real and distinct ($\lambda_1\ne\lambda_2$):

   $$\begin{align}x_1\left(t\right) &= e^{\lambda_1t} \\
   x_2\left(t\right) &= e^{\lambda_2t} \\
   &\hspace{0.555em}\vdots \\
   x\left(t\right) &= Ax_1\left(t\right) + Bx_2\left(t\right)\end{align}$$

2. $\lambda_1$ and $\lambda_2$ are real and equal:

   $$\begin{align}x_1\left(t\right) &= e^{\lambda t} \\
   x_2\left(t\right) &= te^{\lambda t} \\
   &\hspace{0.555em}\vdots \\
   x\left(t\right) &= Ax_1\left(t\right) + Bx_2\left(t\right)\end{align}$$

3. $\lambda_1$ and $\lambda_2$ are complex:

   $$\begin{align}\lambda_2 &= \overline{\lambda_1} \\
     \text{let } \lambda_1 &= p + iq \\
              \therefore \lambda_2 &= p - iq \\
              &\hspace{0.555em}\vdots\\
      x_1\left(t\right) &= e^{pt}e^{iqt} \\
      x_1\left(t\right) &= e^{pt}e^{-iqt} \\
              &\hspace{0.555em}\vdots\\
      x\left(t\right) &= e^{pt}\left[\tilde{A}\cos qt + \tilde{B}\sin qt\right] \\
      \text{where } \begin{bmatrix}\tilde{A}\\ \tilde{B}\end{bmatrix} &= \begin{bmatrix}A+B\\ iA - iB\end{bmatrix}\in\mathbb{R}^2\end{align}$$
**** inhomogenous
$\ddot{x} + a_1\dot{x} + a_0 x = f(t)$
1. find solution of homogenous part, $x_h(t)$
2. find particular solution of inhomogenous equation, $x_p(t)$
3. general solution is $x(t) = x_h(t) + x_p(t)$

To find $x_p(t)$ we assume it is a function of the same type as $f(t)$
1. polynomial of degree n
2. exponential function
3. harmonic $A\cos + B\sin$

* Trig
** Reciprocals

  \begin{array}{ccc|ccc}
    &
      f(x)  &&&
      \frac{1}{f(x)}
    & \\

    \hline

    &
      sin &&&
      cosec
    & \\

    &
      cos &&&
      sec
    & \\

    &
      tan &&&
      cot
    &
  \end{array}
* Series'
** Taylor
*** f(x,y)
Centered at point $(x,y) = (x_0,y_0)$:

$$
  f(x,y) = \sum_{k=0}^\infty \frac{1}{k!}\left(\Delta x\frac{\partial}{\partial x} + \Delta y\frac{\partial}{\partial y}\right)^k f(x_0,y_0)
$$

Of degree $n$:
$$
  f(x,y) = \sum_{k=0}^n \frac{1}{k!}\left(\Delta x\frac{\partial}{\partial x} + \Delta y\frac{\partial}{\partial y}\right)^k f(x_0,y_0) + R_n(x_0,y_0)
$$

$$
  f(x,y) \approx \sum_{k=0}^n \frac{1}{k!}\left(\Delta x\frac{\partial}{\partial x} + \Delta y\frac{\partial}{\partial y}\right)^k f(x_0,y_0)
$$

Where $R_n(x_0,y_0)$ is defined by:

$$
  R_n(x_0,y_0) = \frac{1}n\left(\Delta x\frac{\partial}{\partial x} + \Delta y\frac{\partial}{\partial y}\right)^n f(x+\theta\Delta x,y+\theta\Delta y)
$$

for some constant $\theta\in[0,1]$ and $(\Delta x,\Delta y) = (x-x_0,y-y_0,)$.

* Geometry
** Ellipse
Recall; a circle can be defined as all points a given distance, $r$, from the origin:

$$\left\{(x,y)\in\mathbb{R}^2:\sqrt{x^2 + y^2} = r\in\mathbb{R}\right\}$$

Or for n-dimensions:

$$\left\{\vec{x}\in\mathbb{R}^n:\left\|\vec{x}\right\| = r\in\mathbb{R}\right\}$$

For an ellipse, we define two points, known as foci, $f_1$ and $f_2$. Then the ellipse is defined as all points where the sum of the distance between these two points is fixed:

$$\left\{\vec{x}\in\mathbb{R}^n:\left\|\vec{f}_1 - \vec{x}\right\| + \left\|\vec{f}_2 - \vec{x}\right\| = r\in\mathbb{R}\right\}$$

Also, for $O$ and $O^\prime$ having respective radii of $r$ and $\tilde{r}$, we have:

$$r+\tilde{r} = 2a$$

where $a$ is the semi-major axis.

$2c$ being the distance between the foci, gives:

$$b=\sqrt{a^2 - c^2}$$

for the semi-minor axis.

Perihelion being furthest point on elipse, from center, is $a$.

In polar $(r,\theta)$:

$$r(\theta) = \frac{a^2 - c^2}{a + c\cos\theta} = \frac{l}{1 + \varepsilon\cos\theta}$$

where $l = (a^2 - c^2)/a$, latus rectum, and $\varepsilon=c/a$, and is the excentricity.

* $\LaTeX$
** Augmented Matrices
#+begin_src latex
\newenvironment{amatrix}[1]{%
  \left[\begin{array}{@{}*{#1}|c@{}}
}{%
  \end{array}\right]
}

\begin{amatrix}{ccc|c}
  1 & 2 & 3  & 4 \\
  5 & 6 & 7  & 8
\end{amatrix}
#+end_src
** Gaussian Elimination
*** Tilde
#+begin_src latex
\newenvironment{amatrix}[1]{%

\left[\begin{array}{@{}*{#1}|c@{}}

}{%

\end{array}\right]

}
\begin{align*}

  \begin{amatrix}{ccc|c}
    1 & -2 &  1 & 1 \\
    2 & -1 & -3 & 2 \\
    3 &  0 & -7 & 3
  \end{amatrix}

  & \sim

  \begin{amatrix}{ccc|c}
    1 & -2 &  1  & 1 \\
    2 & -1 & -3  & 2 \\
    0 &  6 & -10 & 0
  \end{amatrix}

  & \begin{array}{c}{R_3 \rightarrow R_3 + (-3)R_1} \\ \end{array} \\

  % - - - - - - - - - - - - - - - - - - - -

  \begin{amatrix}{ccc|c}
    1 & -2 &  1  & 1 \\
    2 & -1 & -3  & 2 \\
    0 &  6 & -10 & 0
  \end{amatrix}

  & \sim

  \begin{amatrix}{ccc|c}
    1 & -2 &  1  & 1 \\
    0 &  3 & -5  & 0 \\
    0 &  6 & -10 & 0
  \end{amatrix}

  & \begin{array}{c}{R_2 \rightarrow R_2 + (-2)R_1} \\ \end{array} \\

  % - - - - - - - - - - - - - - - - - - - -

  \begin{amatrix}{ccc|c}
    1 & -2 &  1  & 1 \\
    0 &  3 & -5  & 0 \\
    0 &  6 & -10 & 0
  \end{amatrix}

  & \sim

  \begin{amatrix}{ccc|c}
    1 & -2 &  1 & 1 \\
    0 &  3 & -5 & 0 \\
    0 &  0 &  0 & 0
  \end{amatrix}

  & \begin{array}{c}{R_3 \rightarrow R_3 + (-2)R_2} \\ \end{array} \\

\end{align*}

\begin{align*}
  \implies 3x_2 - 5x_3 = 0 \\
  3x_2 = 5x_3 \\
  x_2 = \frac{5}{3}x_3
  \text{let } x_3 = \alpha \in \mathbb{R}
  \ldots
  \begin{bmatrix}
    x_1 \\
    x_2 \\
    x_3
  \end{bmatrix} =
  \begin{bmatrix}
    1 + \frac{7}{3}\alpha \\
    \frac{5}{3}\alpha \\
    \alpha
  \end{bmatrix}
\end{align*}
#+end_src
*** Arrow
#+begin_src latex
\newenvironment{amatrix}[1]{%
  \left[\begin{array}{#1}
}{%
  \end{array}\right]
}
\newcommand{\overtext}[2]{\begin{array}{c}#1 \\ #2 \end{array}}

\begin{align}
  \overtext{R_2 \rightarrow R_2 - 4R_1}{
    \begin{amatrix}{cc|c}
      1 & 2  & 3 \\
      4 & 5  & 6
    \end{amatrix}
    \leadsto \begin{amatrix}{cc|c}
      1 & 2  & 3 \\
      0 & -3  & -6
    \end{amatrix}
  }
\end{align}
#+end_src
