#+TITLE:Physics Cheatsheet
#+AUTHOR:LiquidZulu
#+HTML_HEAD:<link rel="stylesheet" type="text/css" href="file:///e:/emacs/documents/org-css/css/org.css"/>
#+OPTIONS: ^:{}
#+STARTUP: latexpreview
#+begin_comment
/This file is best viewed in [[https://www.gnu.org/software/emacs/][emacs]]!/
#+end_comment

* Photonics and Optics
** Snell's Law
For monochromatic light in a given material, snells law states:

$$
  \frac{\sin{\theta_2}}{\sin{\theta_1}} = \frac{v_2}{v_1} = \frac{n_1}{n_2}
$$

Where $\theta$ is the angle measured from the normal to the ray, $v$ is the velocity of light in the respective medium, and $n$ is the refractive index of the respective medium.

#+CAPTION:Refraction of light at the interface between two media of different refractive indices, with n2 > n1. Since the velocity is lower in the second medium (v2 < v1), the angle of refraction θ2 is less than the angle of incidence θ1; that is, the ray in the higher-index medium is closer to the normal.
[[./images/snells-law.png]]
** Malus' Law
$\begin{array}{c} A = A_0 \cos{\theta} \\ I \propto A^2 \\ A^2 = {A_0}^2 \cos^2{\theta}\end{array}$

Gives us Malus' Law:
$I = I_0 \cos^2{\theta}$

Where $\theta$ is the angle of the second polarising filter, $I$ is the intensity of light coming out of that filter, and $I_0$ is the initial intensity, that is, the intensity of polarised light going into the second filter.
** Brewster's Angle
Brewster's angle (also known as the polarization angle) is an angle of incidence at which light with a particular polarization is perfectly transmitted through a transparent dielectric surface, with no reflection. When /unpolarized/ light is incident at this angle, the light that is reflected from the surface is therefore perfectly polarized.

$\theta_B = \arctan{\frac{n_2}{n_1}}$
Where $\arctan{x}$ is the inverse tangent of $x$, and $n_a$ is the refractive index of $a$.
** curved refractive surface
*** Thick lens equation (f, n_lens, R_1, R_2, t)
$\frac{1}{f} = \left(n_{lens} - 1\right)\left[\frac{1}{R_1} - \frac{1}{R_2} + \frac{\left(n_{lens} - 1\right)t}{n_{lens}R_1 R_2}\right]$
+ $f$ - The focal point from the rear principle plane
+ $n_{lens}$ - The refractive index of the lens
+ $R_1$ The radius of curvature of the front surface
+ $R_2$ The radius of curvature of the rear surface
+ $t$ -  The thickness of the lens
*** thin lens equation (f, n_lens, n_material, R_1, R_2, s_o, s_i)
also called lensmakers equation, thin lens is a good approximation:

$\frac{1}{f} = \left(n_{lens} - 1\right)\left[\frac{1}{R_1} - \frac{1}{R_2}\right]$

or immersed in some non-air or non-vacuum:

$\frac{1}{f} = \left(\frac{n_{lens}}{n_{material}} - 1\right)\left[\frac{1}{R_1} - \frac{1}{R_2}\right]$

*** paraxial equation (n_1, n_2, s_o, s_i, R)
$\frac{n_1}{s_o} + \frac{n_2}{s_i} = \frac{n_2 - n_1}{R}$
*** focal length
**** single curved surface (f_o, f_i, n_1, n_2, R)
when object sits on focal point s_i goes to infinity (far field)
$f_o = \frac{n_1 R}{n_2 - n_1}$

when object at infinity rays converge at focal point
$f_i = \frac{n_2 R}{n_2 - n_1}$
**** lens
***** back focal length (f, n_l, t, f, R_1)
bfl is farfield light being focused to a point

$bfl = f - \frac{\left(n_l - 1\right)tf}{n_l R_1}$

or for multiple lenses:
$bfl = \frac{f_2 \left(d - f_1\right)}{d - \left(f_1 + f_2\right)}$
***** front focal length (f, n_l, t, f, R_2)
ffl is an object at the focal point being columnated

$ffl = f - \frac{\left(n_l - 1\right)tf}{n_l R_2}$

or for multiple lenses:
$ffl = \frac{f_1 \left(d - f_2\right)}{d - \left(f_1 + f_2\right)}$
***** effective focal length
As distance goes to zero it becomes easy to calculate
$\frac{1}{efl} = \frac{1}{f_1} + \frac{1}{f_2} - \frac{d}{f_1 f_2}$

*** lateral magnification (n_1, n_2, y_1, y_2, s_o, s_i, m)

$n_1 \frac{y_1}{s_o} = -n_2 \frac{y_2}{s_i}$

where y_1 is the object and y_2 is the image of that object. right hand side negative as its upside down

$\frac{y_2}{y_1} = m = - \frac{n_1 s_i}{n_2 s_o}$

for thick lenses:
$M = \frac{y_i}{y_o} = -\frac{s_i}{s_o}$

for multiple lenses close together:
$M_1 = -\frac{f_1}{s_{o_1} - f_1}$

$M_2 = -\frac{s_{i_2}}{d - s_{i_1}}$

$M_T = M_1 M_2$
*** angular magnification
$M_\theta = \frac{\theta_e}{\theta_o} = \frac{\left(\frac{h}{f_e}\right)}{\left(\frac{h}{f_o}\right)} = \frac{f_o}{f_e} = \frac{f_1}{f_2}$
*** gaussian lens formula (s_o, s_i and f)
For a thick lens:
$\frac{1}{s_o} + \frac{1}{s_i} = \frac{1}{f}$
*** sign convention
[[./images/optics-sign-convention.png]]
[[./images/optics-sign-convention-thick.png]]
*** lens power
the degree to which a refractive lens, reflective mirror, or combined optical system converges or diverges light, measured in dioptre or $m^{-1}$:

$P = \frac{1}{f}$
*** telescope fov
[[./images/telescope-fov.png]]
*** two lenses close together
$$
  s_{i_2} = \frac{
    f_2 d - f_2\left[\frac{
      s_{o_1} f_1
    }{
      s_{o_1} - f_1
    }\right]
  }{
    d - f_2 - \left[\frac{
      s_{o_1} f_1
    }{
      s_{o_1} - f_1
    }\right]
  }$$
*** diagrams
Thick lens:
[[./images/thick-lens-diagram.png]]
** curved reflective surface
*** focal length
$f=-\frac{R}{2}$
concave: negative because R is negative, due to being on the left, so f is positive
convex: R pos so f negative, defocuses
*** object and image distance
$\frac{1}{s_o} + \frac{1}{s_i} = \frac{1}{f} \therefore \frac{1}{s_o} + \frac{1}{s_i} = -\frac{2}{R}$
*** magnification
$M_T = \frac{y_i}{y_o} = -\frac{s_i}{s_o}$
*** ray diagrams
[[./images/optics-mirror-ray-diagrams.png]]
*** sign convention
[[./images/optics-sign-convention-mirror.png]]
[[./images/optics-sign-convention-mirror-2.png]]
** optical aberrations
[[./images/optical-aberrations.png]]
$\nu$ is abbe number:
[[./images/abbe-number.png]]
** Wave Optics
*** refractive index derivation
$$n=\frac{c}{v}$$
*** Plane wave equation (electric field)
$\operatorname{E}(x,t) = E_0\cos(kx-\omega t + \varphi_1)$

$$\vec{E} = \vec{E}_0\cdot\cos(\vec{k}\cdot\vec{r}-\omega t + \varphi)$$

$$\operatorname{E}(x,t) = E_0\cos(kx - \omega t + \varphi_1) = Re\left[E_0 e^{i(kx - \omega t + \varphi_1)}\right]$$ <- because eulers formula

$$\tilde{E} = E_0 e^{i(kx - \omega t + \varphi_1)} \implies E=\tilde{E}+ \overline{\tilde{E}}$$
**** wavenumber
$$k = \frac{\tau}{\lambda}n$$
n refractive index
**** angular frequency
$$\omega = \tau f = \frac{\tau}{T}$$
**** ang freq / wavenumber = speed of light
$$\frac{\omega}{k} = \lambda f = c$$
*** Intensity
$$I=\frac{1}{2}\cdot n\cdot \varepsilon_0\cdot  c\cdot  {E_0}^2 \implies I \propto {E_0}^2$$
*** Superposition
$$\begin{align}\begin{aligned}
    \operatorname{E}_T(z,t) &= E_0\sin(\omega t + \alpha_R) \\
    {E_0}^2 &= {{E_0}_1}^2 + {{E_0}_2}^2 + 2{{E_0}_1}{{E_0}_2}\cos(\alpha_1 - \alpha_2)
  \end{aligned}
  & \leadsto \begin{cases}
    \operatorname{E}_1(\omega) + \operatorname{E}_2(\omega) = \operatorname{E}_T(\omega)& \\
    \alpha_R = \alpha_R((\alpha_1 - \alpha_2), E_1, E_2)& \\
    E_T = E_T((\alpha_1 - \alpha_2), E_1, E_2)& \\
    \alpha_1 - \alpha_2 = (2m)\pi &\rightarrow \begin{array}{ccc}{{E_0}_{\text{max}}}^2  & \widehat{=} & \text{Constructive interference} \end{array} \\
    \alpha_1 - \alpha_2 = (2m + 1)m &\rightarrow \begin{array}{ccc} {{E_0}_{\text{min}}}^2 & \widehat{=} & \text{Destructive interference} \end{array} \\
  \end{cases}
\end{align}$$

counterpropagating waves in cavity:
$$E_T(z,t) = 2{E_0}_1\sin(kz)\cos(\omega t)$$

waves with different frequencies:

$$\begin{array}{c}
  \bar{k}:= \frac{k_1 + k_2}{2},\bar{\omega}:= \frac{\omega_1 + \omega_2}{2},k_m:= \frac{k_1 - k_2}{2},\omega_m:= \frac{\omega_1 - \omega_2}{2} \\ \\ \\
  E_T(z,t) = 2{E_0}_1\cos(\bar{k}z - \bar{\omega}t)\cos(k_m z - \omega_m t)
\end{array}$$
*** polarization of light
if:

$${E_0}_x = {E_0}_y = {E_0}$$
$$\Delta\varphi=\pm m\pi$$

Then the polarization is linear at $45^\circ$. +ve for $\Delta\varphi=\pm 2m\pi$, and -ve for $\Delta\varphi=\pm(2m + 1)\pi$

if:

$${E_0}_x \ne {E_0}_y$$
$$\Delta\varphi=\pm m\pi$$

Then the polarization is linear forming an angle $\alpha$:

$$\alpha=\tan^{-1}\frac{{E_0}_y}{{E_0}_x}$$

if:

$${E_0}_x = {E_0}_y = E_0$$
$$\Delta\varphi=\pm \frac{\pi}{2}$$

Then the polarisation is circular, -ve right handed and +ve left handed.

if:

$${E_0}_x \ne {E_0}_y$$
$$\Delta\varphi\ne\pm m\pi$$

Then the electric field draws an ellipse, making an angle $\psi$ with the x-axis:

$$\tan 2\psi = \frac{2{E_0}_x{E_0}_y\cos\varphi}{{E_0}_x^2-{E_0}_y^2}$$

**** Fermat's principle

Light propogates along the path that minimises the integral:

$$t = \frac{1}{c}\int_A^B n\text{d}s$$

It gives snells law as:

$$n_i\sin\theta_i = n_t\sin\theta_t$$

Fresnels coefficients:

[[./images/fresnel-coeffs.png]]
[[./images/fresnel-coeffs-1.png]]
[[./images/fresnel-coeffs-2.png]]
[[./images/fresnel-coeffs-3.png]]
[[./images/fresnel-coeffs-4.png]]
*** coherence, interference and diffraction
**** coherence
[[./images/temporal-coherence.png]]
[[./images/temporal-coherence-1.png]]


[[./images/spatial-coherence.png]]

**** diffraction
[[./images/diffraction-A.png]]
[[./images/diffraction-B.png]]

**** Interference
***** Youngs double slit
[[./images/double-slit.png]]
***** Lloyd's interferometer
[[./images/lloyd-interferometer.png]]
***** Michelson interferometer
[[./images/michelson-interferometer.png]]
***** Mach-Zehnder interferometer
[[./images/mach-interferometer.png]]
***** Fabry-Perot interferometer (etalon)
[[./images/fabry-interferometer.png]]
[[./images/fabry-interferometer-1.png]]
[[./images/fabry-interferometer-2.png]]
*** Laser Physics
[[./images/laser-0.png]]


[[./images/laser-1.png]]


[[./images/laser-2.png]]


[[./images/laser-3.png]]


[[./images/laser-4.png]]


[[./images/laser-5.png]]


[[./images/laser-6.png]]


[[./images/laser-7.png]]


[[./images/laser-8.png]]
*** Fiber Optics
[[./images/fiber-optics-0.png]]


[[./images/fiber-optics-1.png]]


[[./images/fiber-optics-2.png]]


[[./images/fiber-optics-3.png]]


[[./images/fiber-optics-4.png]]


[[./images/fiber-optics-5.png]]


[[./images/fiber-optics-6.png]]
* Dynamics
** Newtons Laws
*** First Law body in motion
$F = 0 \implies a = 0$
*** Second Law rate of change of momentum is equal to the force acting on it
$\frac{dP}{dt} = F$
** Kepplers laws
*** first law
orbit of a planet is an ellipse:

$$r=\frac{l}{1+\varepsilon\cos\theta}$$

Furthermore we get a formula for eccentricity and the latus rectum:

$$l=\frac{L^2}{m\alpha}$$

$$\varepsilon = \sqrt{1+\frac{2EL^2}{\alpha^2m}}$$

Where:

$E = \frac{1}{2}m\|\dot{\vec{r}}\|^2 + V(\vec{r})$
$L = mr^2\dot{\theta}$
$\alpha = GM_\text{sun}m$

*** second
planet sweeps out equal area in an equal interval of time:

$$\frac{\text{d}A}{\text{d}t} = \frac{r^2}{2}\frac{\text{d}\theta}{\text{d}t} = \frac{abn}{2} = \frac{\pi ab}{P}$$

Where $n$ is the mean motion and $P$ is the period:

$$n = \frac{2\pi}{P}$$

*** third
The ratio of the square of an object's orbital period with the cube of the semi-major axis of its orbit is the same for all objects orbiting the same primary.

$$\frac{a^3}{T^2} = \frac{G(M + m)}{4\pi^2} \approx \frac{GM}{4\pi^2}$$

for $m\ll M$.

Alternatively, for the solar system specifically:

$$T^2 = \frac{4\pi^2a^3}{GM_\text{sun}}$$

** Simple Harmonic Motion
*** Hook's Law
$F_H = k\cdot x$
where k is the spring constant in n/m or kg/s^2

$m \ddot{x} = -k x$

$\omega = \sqrt{\frac{k}{m}}$
where \omega is the angular frequency

$\ddot{x} = -\omega^2 x$

solutions:
$$\begin{array}{c}
  x\left(t\right) =  \cos \left(\omega t\right) \\
  x\left(t\right) =  \sin \left(\omega t\right)
\end{array}$$

principle of superpositions:
if $x_1 \left(t\right)$ and $x_2 \left(t\right)$ are solutions to $m \ddot{x} = -k x$ then so are arbitrary linear combinations of $x_1$ and $x_2$:

$x\left(t\right) = A x_1 \left(t\right) + B x_2 \left(t\right)$

That is to say:
$x\left(t\right) = A \cos \left(\omega t\right) + B \sin \left(\omega t\right)$

knowing $x\left(0\right)$ and $\dot{x}\left(0\right)$ allows you to solve
*** Amplitude
$$\begin{align}
  A \cos \left(\omega t\right) + B \sin \left(\omega t\right) &= R\cos\left(\omega t - \Phi\right) \\
  \cos\left(\alpha - \beta\right) &= \cos\left(\alpha\right)\cos\left(\beta\right) + \sin\left(\alpha\right)\sin\left(\beta\right) \\
  &\vdots \\
  A &= R\cos\Phi \\
  B &= R\sin\Phi \\
  &\vdots \\
  R &= \sqrt{A^2 + B^2} \\
  \frac{B}{A} &= \tan\Phi \\
\end{align}$$

Where R is the amplitude
*** Period
$T = \frac{2\pi}{\omega}$
*** Energy
**** Angular
***** Kinetic
$$K=\frac{1}{2}m\left\langle\dot{\vec{r}},\dot{\vec{r}}\right\rangle = \frac{1}{2}m\dot{r}^2 + \frac{L^2}{2mr^2}$$

where $L= mr^2\dot{\theta}^2$
**** Potential
$V = \frac{1}{2} k x^2$
**** Total
$E = \frac{1}{2}m\dot{x}^2 + \frac{1}{2}kx^2 = K + V$
**** Average energies
$$\begin{align}
K_{av} &= \frac{1}{T} \int_0^T \left. \frac{1}{2} m \dot{x}^2 \right. dt \\
V_{av} &= \frac{1}{T} \int_0^T \left. \frac{1}{2} k x^2 \right. dt\end{align}$$
** oscillations with damping
${\omega_0}^2 = \frac{k}{m}, \gamma = r/m$
$F_{damping} = -vr$
$\leadsto m\ddot{x} = \underbrace{-\dot{x}r}_{\text{damping}} \underbrace{-kx}_{\text{elastic}} + \underbrace{f(t)}_{\text{other}}$

f(t) = 0:
$\ddot{x} + \gamma\dot{x} + {\omega_0}^2x = 0$
$\leadsto \lambda^2 + \gamma\lambda + {\omega_0}^2 = 0$

*** underdamped case
$\gamma^2 < 4\omega_0^2$
$\lambda_1 = -\gamma/2 + i\beta$

$\lambda_2 = \bar{\lambda_1}$

where $\beta = \sqrt{{\omega_0}^2 - \gamma^2/4}\in\mathbb{R}$

generally:
$x(t) = e^{-(\gamma/2) t} (Ae^{i\beta t} + Be^{-i\beta t})$
or:
$x(t) = e^{-(\gamma/2) t}R\cos(\beta t - \phi)$ <- amplitude exponentially decreasing
*** overdamped case
$\gamma^2 > 4\omega_0^2$

$x(t) = Ae^{\lambda_1 t} + Be^{\lambda_2 t}$
*** critically damped
$\gamma^2 = 4\omega_0^2$

$x(t) = (A + Bt)e^{-(\gamma/2)t}$
** forced oscillator
$\ddot{x} + \gamma\dot{x} + {\omega_0}^2 = \frac{f_0}{m}\cos(\omega t)$

for f_0 = 0 x(t) would tend to 0, not when f is nonzero

look at a particular solution:
$$\begin{align}
  x_p(t) &= C\cos(\omega t) + D\sin(\omega t) \\
  \dot{x}_p(t) &= -\omega C\sin(\omega t) + \omega D\cos(\omega t) \\
  \ddot{x}_p(t) &= -\omega^2 C\cos(\omega t) - \omega^2 D\sin(\omega t)
\end{align}$$

sub into equation of motion:
+ At cos: $-\omega^2C + \gamma D \omega + {\omega_0}^2C = \frac{f_0}{m}$
+ At sin: $-\omega^2D + \gamma C \omega + {\omega_0}^2D = 0$

Consider these as simultaneous equations, giving:

$$\begin{align}
  D &= \frac{f_0 \gamma \omega}{m\left[({\omega_0}^2 - {\omega}^2)^2 + \gamma{\omega}^2\right]} \\
  C &= \frac{f_0 ({\omega_0}^2 - {\omega}^2)}{m\left[({\omega_0}^2 - {\omega}^2)^2 + \gamma{\omega}^2\right]} \\
  x_p(t) &= C\cos(\omega t) + D\sin(\omega t) \\
  x_p(t) &= R\cos(\omega t - \phi) \\
  R &= \frac{f_0}{m\sqrt{({\omega_0}^2 - {\omega}^2)^2 + \gamma{\omega}^2}} \\
  \tan(\phi) &= \frac{D}{C} = \frac{\gamma\omega}{{\omega_0}^2 - \omega^2}
\end{align}$$


$x_p(t)$ describes the steady state of the system at large t
** 3D Kinematics
*** Position
Use vectors
$\vec{v} = \overrightarrow{OP}$ for point P from origin

**** angle
$\vec{r}_1 \cdot \vec{r}_2 = \lVert\vec{r}_1\rVert\lVert\vec{r}_2\rVert\cos(\phi)$
*** velocity/accel as a vector
$\vec{v} = \dot{x}\hat{\imath} + \dot{y}\hat{\jmath} + \dot{z}\hat{k}$
$\Delta\vec{r}(t) = \vec{r}(t + \Delta t) - \vec{r}(t)$
$\vec{v}(t) = \dot{\vec{r}}(t) = \underset{\Delta t \to 0}{\lim}\frac{\vec{r}(t+\Delta t) - \vec{r}(t)}{\Delta t}$

$v = \lVert\vec{v}\rVert$
$v_x = \dot{x} = \frac{dx}{dt}$

$\vec{a} = \dot{\vec{v}}$
*** integrating vectors
$$\begin{align}
  \vec{v}(t) &= 2\hat{e}_1 + 2t\hat{e}_2 -3t^2\hat{e}_3 \\
  \vec{r}(t) &= 2t\hat{e}_1 + t^2\hat{e}_2 - t^3\hat{e}_3 + \vec{c}
\end{align}$$

with a vector rather than a scalar constant

** Momentum
*** Angular
$$\lVert\vec{a}\times\vec{b}\rVert = \lVert\vec{a}\rVert\lVert\vec{b}\rVert\sin\theta$$

Direction is perpendicular to both a and b, clockwise inwards, anti-clockwise outwards

$$\begin{align}
  \hat{\imath}\times\hat{\jmath} &= \hat{k} \\
  &\hspace{0.555em}\vdots \\
  \vec{x}\times\vec{y}&=\begin{vmatrix}
    \hat{e}_1 & \hat{e}_2 & \hat{e}_3 \\
    x_1 & x_2 & x_3 \\
    y_1 & y_2 & y_3 \\
  \end{vmatrix}
\end{align}$$


Angular momentum is given by:

$$\overrightarrow{L} = m\vec{r}\times\dot{\vec{r}} = m\vec{r}\times\vec{v}$$

$\vec{r}$ is position vector and $\dot{\vec{r}}$ is velocity vector.

For polar coordinates, $(r,\theta)$:

$$\vec{r} = r\cos\theta\hat{e}_1+r\sin\theta\hat{e}_2$$

$$r=r(t),\theta=\theta(t)$$

$$\dot{\vec{r}} = (\dot{r}\cos\theta - r\dot{\theta}\sin\theta)\hat{e}_1 + (\dot{r}\sin\theta + r\dot{\theta}\cos\theta)\hat{e}_2$$

We also have:
$$\overrightarrow{L} = m\vec{r}\times\dot{\vec{r}} = m\vec{r}\times\vec{v} = m\hat{e}_3\big(r\cos\theta\cdot(\dot{r}\sin\theta + r\dot{\theta}\cos\theta) - r\sin\theta\cdot(\dot{r}\cos\theta - r\dot{\theta}\sin\theta)\big)$$

$$\leadsto\overrightarrow{L} = mr^2\dot{\theta}\hat{e}_3$$

Only angular velocity, $\dot{\theta}$, contributes to momentum, but not the radial velocity, $\dot{r}$.

And the expression for the magnitude is trivially:

$$\left\|\overrightarrow{L}\right\| = mr^2\dot{\theta}$$
**** Conservation
$$\frac{\text{d}}{\text{d}t}(\vec{a}\times\vec{b}) = \dot{\vec{a}}\times\vec{b} + \vec{a}\times\dot{\vec{b}}$$

$$\frac{\text{d}}{\text{d}t}\overrightarrow{L} = m\frac{\text{d}}{\text{d}t}(\vec{r}\times\dot{\vec{r}}) = m(\vec{r}\times\ddot{\vec{r}})$$

$$m\ddot{\vec{r}} = \overrightarrow{F} \implies \frac{\text{d}}{\text{d}t}\overrightarrow{L} = \vec{r}\times\overrightarrow{F}$$

If the force acting on the particle can be written as $\overrightarrow{F} = f\left(\left\|\vec{r}\right\|\right)\vec{r}$, where $f$ is some function, then $\frac{\text{d}\overrightarrow{L}}{\text{d}t} = 0$, i.e. $\overrightarrow{L}$ is conserved. These are called central forces.
+ gravity is an example:

  $$\overrightarrow{F}_g = -\frac{GmM}{r^3}\vec{r} = f\left(r\right)\vec{r} = f\left(\left\|\vec{r}\right\|\right)\vec{r}$$
** Conservation of Energy
$$f=f(x,y,z)$$
$$\nabla f(\vec{r}) = \frac{\partial f}{\partial x}\hat{\imath} + \frac{\partial f}{\partial y}\hat{\jmath} + \frac{\partial f}{\partial z}\hat{k}$$

Or generally:
$$\nabla f(\vec{x}) = \sum_{k=1}^n\frac{\partial f}{\partial x_k}\hat{e}_k = \left[\sum_{k=1}^n\frac{\partial}{\partial x_k}\hat{e}_k\right]\cdot f(\vec{x})$$

We say that a force $\overrightarrow{F}$ is conservative if it can be written as:
$$\overrightarrow{F} = -\nabla V$$

Where $V = V(x,y,z)$ is called the potential energy of $\overrightarrow{F}$

For a particle of mass $m$ and position $\vec{r}(t)$, moving according to Newton's Second Law under the influence of conservative force with potential $V(\vec{r})$, the total energy:

$$E=\frac{1}{2}m\left\|\dot{\vec{r}}\right\|^2 + V(\vec{r})$$

is conserved.
